compiler/backend/proofs/source_to_modProofScript.sml
@@ -275,7 +275,7 @@ val (s_rel_rules, s_rel_ind, s_rel_cases) = Hol_reln `
   (!s s'.
     LIST_REL (sv_rel s'.globals) s.refs s'.refs ∧
     s.defined_types = s'.defined_types ∧
-    s.defined_mods = IMAGE (\x. [x]) s'.defined_mods ∧
+    s.defined_mods = s'.defined_mods ∧
     s.clock = s'.clock ∧
     s.ffi = s'.ffi
     ⇒
@@ -302,7 +302,8 @@ val match_result_rel_def = Define
 val invariant_def = Define `
   invariant var_map env s s_i1 ⇔
     global_env_inv s_i1.globals var_map {} env ∧
-    s_rel s s_i1`;
+    s_rel s s_i1 ∧
+    [] ∉ s.defined_mods`;
 
 val invariant_change_clock = Q.store_thm("invariant_change_clock",
   `invariant menv env st1 st2 ⇒
@@ -1935,7 +1936,7 @@ val no_dup_types_dec = Q.prove (
   simp []);
 
 val invariant_defined_mods = Q.prove(
-  `invariant c d e f ⇒ e.defined_mods = IMAGE (\x. [x]) f.defined_mods`,
+  `invariant c d e f ⇒ e.defined_mods = f.defined_mods`,
   rw[invariant_def,s_rel_cases]);
 
 val invariant_defined_types = Q.prove(
@@ -2088,8 +2089,11 @@ val compile_prog_correct = Q.store_thm ("compile_prog_correct",
         fs [s_rel_cases, update_mod_state_def] >>
         drule evaluate_decs_globals >>
         rw [] >>
-        fs []))
+        fs [])
+      >- (fs [s_rel_cases] >> metis_tac [evaluate_decs_state_const, FST])
+      >- (fs [s_rel_cases] >> metis_tac [evaluate_decs_state_const, FST]))
     >- (
+      `[] ∉ s_i1.defined_mods` by (fs [s_rel_cases] >> metis_tac [evaluate_decs_state_const, FST]) >>
       fs [s_rel_cases, update_mod_state_def, result_rel_cases] >>
       metis_tac [v_rel_weakening]))
   (* Module case *)
@@ -2113,11 +2117,7 @@ val compile_prog_correct = Q.store_thm ("compile_prog_correct",
     strip_tac >>
     drule prompt_mods_ok >>
     drule no_dup_types >>
-    `mn ∉ s_i1.defined_mods`
-      by (
-        fs [s_rel_cases] >>
-        `[mn] ∉ IMAGE (\x. [x]) s_i1.defined_mods` by metis_tac [] >>
-        fs []) >>
+    `[mn] ∉ s_i1.defined_mods` by (fs [s_rel_cases] >> metis_tac []) >>
     simp [] >>
     Cases_on `result` >>
     fs [] >>
@@ -2132,8 +2132,9 @@ val compile_prog_correct = Q.store_thm ("compile_prog_correct",
       fs [s_rel_cases, update_mod_state_def] >>
       drule evaluate_decs_globals >>
       rw [] >>
-      fs [])
-    >- fs [s_rel_cases, update_mod_state_def]
+      fs [GSYM INSERT_SING_UNION])
+    >- (fs [s_rel_cases] >> metis_tac [evaluate_decs_state_const, FST])
+    >- fs [s_rel_cases, update_mod_state_def, GSYM INSERT_SING_UNION]
     >- (
       fs [s_rel_cases, update_mod_state_def, result_rel_cases] >>
       metis_tac [v_rel_weakening])));
@@ -2144,7 +2145,7 @@ val compile_prog_mods = Q.prove (
     ⇒
     semanticPrimitives$prog_to_mods prog
     =
-    MAP (\x. [x]) (modSem$prog_to_mods prog_i1)`,
+    modSem$prog_to_mods prog_i1`,
   induct_on `prog` >>
   srw_tac[][compile_prog_def, LET_THM, modSemTheory.prog_to_mods_def, semanticPrimitivesTheory.prog_to_mods_def] >>
   srw_tac[][] >>
@@ -2159,7 +2160,10 @@ val compile_prog_mods = Q.prove (
   fs [] >>
   first_x_assum drule >>
   rw [] >>
-  fs [semanticPrimitivesTheory.prog_to_mods_def, modSemTheory.prog_to_mods_def]);
+  fs [semanticPrimitivesTheory.prog_to_mods_def, modSemTheory.prog_to_mods_def] >>
+  Cases_on `p'` >>
+  fs [] >>
+  rw []);
 
 val compile_prog_top_types = Q.prove (
   `!l var_map prog l' var_map' prog_i1.
@@ -2245,7 +2249,7 @@ open semanticsTheory
 val precondition_def = Define`
   precondition s1 env1 conf s2 env2 ⇔
     invariant conf.mod_env env1.v s1 s2 ∧
-    IMAGE (\x. [x]) s2.defined_mods = s1.defined_mods ∧
+    s2.defined_mods = s1.defined_mods ∧
     s2.defined_types = s1.defined_types ∧
     env2.c = env1.c ∧
     env2.v = [] ∧
